new theorems

typedLambda.v
@@ -1,4 +1,8 @@
-Require Import ssreflect List.
+Require Import ssreflect Arith.
+Require Import Arith.EqNat.
+Require Import Arith.Compare_dec.
+Require Import List.
+Require Import Omega.
 
 Inductive typ :=
   | Tnat : typ
@@ -14,7 +18,35 @@ Check nth.
 Check (list).
 Definition context (t: Set) := list (option t).
 
-Fixpoint omap (ty: typ) (oty: option typ) : option typ:=
+
+Lemma lambda_equivalence: forall (t u: term) (ty: typ), t = u <-> (Lambda ty t = Lambda ty u).
+Proof.
+  move => t u.
+  split;(move => h0).
+  rewrite h0.
+  done.
+  inversion h0.
+  trivial.
+Qed.
+
+Lemma app_equivalence: forall t u v w: term, App t u = App v w <-> (t = v) /\ (u = w).
+Proof.
+  move => t u v w.
+  split.
+  move => h0.
+  split.
+  inversion h0.
+  done.
+  inversion h0.
+  done.
+  move => [h0 h1].
+  rewrite h0.
+  rewrite h1.
+  done.
+Qed.
+
+
+Fixpoint omap (oty: option typ)  (ty: typ) : option typ:=
   match oty with
     | None => None
     | Some t => Some (Tarrow (ty) (t)) 
@@ -28,11 +60,193 @@ Fixpoint type (ctx: list typ) (t: term) : option typ :=
                      if type ctx t2 is Some t1l then Some t1r
                      else None
                    else None
-    | Lambda ty t => omap ty (type (ty :: ctx) t) 
+    | Lambda ty t => omap (type (ty :: ctx) t) ty
   end.
 
-(*Inductive well_typed : list typ -> term -> Prop :=
-| var_is_well : forall (n: nat) (l: list typ), n < length l -> well_typed l (Var n)
-| const_is_well : forall (n:nat) (l: list typ), well_typed l (ConstNat n)
-| app_is_well : forall (t u: term) (ty: typ) (l: list typ), well_typed (Lambda ty t) -> well_typed u -> well_typed (App (Lambda ty t) u)
-| lambda_is_well : forall (t: term) (ty: typ) (l: list typ), well_typed t -> well_typed (Lambda ty t).*)
+
+Fixpoint C (i: nat) (t: term): Prop :=
+  match t with
+    | Var v => (v < i)
+    | ConstNat v => True
+    | App t1 t2 => (C i t1) /\ (C i t2)
+    | Lambda ty t1 => C (i+1) t1
+  end.
+
+(*Question 1.2*)
+Lemma ind_C_pred: forall t: term, forall n: nat, C n t -> C (n+1) t.
+Proof.
+  induction t; simpl; intros.
+  omega; trivial.
+  trivial.
+  split.
+  apply IHt1.
+  by destruct H.
+  apply IHt2. by destruct H.
+  by apply IHt.
+Qed.
+
+
+Fixpoint lifting (n: nat) (k: nat) (t: term): term :=
+  match t with
+    | Var i => if leb k i then Var (i+n) else Var i
+    | ConstNat i => ConstNat i
+    | App t1 t2 => App (lifting n k t1) (lifting n k t2)
+    | Lambda ty t1 => Lambda ty (lifting n (k+1) t1)
+  end.
+
+Fixpoint substitution (i: nat) (t1: term) (t2: term): term :=
+  match t1 with
+    | Var v => if beq_nat i v then t2 else Var v
+    | ConstNat i => ConstNat i
+    | App t3 t4 => App (substitution i t3 t2) (substitution i t4 t2)
+    | Lambda ty t3 => Lambda ty (substitution (i+1) t3 (lifting 1 0 t2))
+  end.
+
+
+(*Question 1.4.2*)
+Theorem no_index_sub: forall (t u: term) (i: nat), (C i t) -> substitution i t u = t.
+Proof.
+  induction t; simpl; intros.
+  have:(beq_nat i n = false).
+  apply beq_nat_false_iff.
+  omega.
+  move => h0.
+  by rewrite h0.
+  trivial.
+  rewrite app_equivalence; split.
+  apply IHt1.
+  apply H.
+  apply IHt2.
+  apply H.
+  apply lambda_equivalence.
+  by apply IHt.
+Qed.
+
+Definition has_type (ctx: list typ) (t: term) := exists ty: typ, type ctx t = Some ty.
+
+Lemma nth_of_list: forall (A: Type) (l: list A) (n: nat), n < length l <-> exists a: A, nth_error l n = Some a. 
+Proof.
+  intros A l.
+  split.
+  move: n.
+  induction l; simpl.
+  intros; omega.
+  intro; case n; simpl.
+  intros.
+  exists a.
+  done.
+  intros.
+  apply IHl.
+  omega.
+  intro h0.
+  case:h0.
+  move: n.
+  induction l; simpl.
+  intros.
+  have:nth_error nil n = None.
+  intros.
+  induction n.
+  by simpl.
+  by simpl.
+  intro.
+  by rewrite x0 in p.
+  intro.
+  case:n; simpl.
+  intros.
+  omega.
+  intros.
+  have: n < (length l) -> S n < S (length l).
+  omega.
+  intro h0; apply h0.
+  by apply (IHl _ x).
+Qed.
+
+Lemma app_is_typed: forall (t1 t2: term) (ctx: list typ), has_type ctx (App t1 t2) -> has_type ctx t1 /\ has_type ctx t2.
+Proof.
+  unfold has_type.
+  intros.
+  split.
+  case H.
+  intro.
+  simpl.
+  case (type ctx t1).
+  intros.  
+    by exists t.
+  intros.            
+  by exists x.
+  case H.
+  simpl.
+  case (type ctx t2).
+  case (type ctx t1).
+  intro.
+  case t.
+  intros.
+  done.
+  intros.
+  by exists t4.
+  intros.
+  done.
+  case (type ctx t1).
+  intro.
+  case t.
+  done.
+  done.
+  done.
+Qed.  
+
+Lemma omap_eq: forall (oty: option typ) (ty: typ), (exists t0:typ, omap oty ty = Some t0) -> (exists t1:typ, oty = Some t1).
+Proof.
+  intros.
+  case:H.
+  intro.
+  unfold omap.
+  case oty.
+  intros.
+  by exists t.
+  done.
+Qed.
+
+
+(*The converse is not true*)
+Lemma typable_implies_closed: forall (t: term) (ctx: list typ), has_type ctx t -> C (length ctx) t.
+Proof.
+  induction t; simpl.
+  unfold has_type.
+  simpl.
+  intros.
+  case H.
+  intros.
+  induction ctx; simpl.
+  have:nth_error nil n = None.
+  intros.
+  induction n.
+  by simpl.  simpl.
+  by simpl.
+  intro h0.
+  by rewrite h0 in H0.  
+  apply nth_of_list in H.
+  done.
+  intro.
+  done.
+  unfold has_type.
+  intros.
+  case H.
+  intros.
+  split.
+  apply IHt1.
+  apply (app_is_typed t1 t2 ctx).
+  done.
+  apply IHt2.
+  by apply (app_is_typed t1 t2 ctx).
+  intro.
+  unfold has_type.
+  simpl.
+  intros.
+  case:H.
+  intros x H0.
+  rewrite plus_comm.
+  apply (IHt (t::ctx)).
+  unfold has_type.
+  apply (omap_eq _ t).
+  by exists x.
+Qed.
